$$
\begin{align}
y^2 - 6y + 24x - 111 &= 0 \\
y^2 -6y + 9 - 9 + 24x - 111 &= 0 \\
(y^2 -6y + 9) + 24x - 120 &= 0 \\
(y-3)^2 + 24x - 120 &= 0 \\
(y-3)^2 &= -24x + 120 \\
(y-3)^2 &= -24(x-5) \\
(y-3)^2 &= 4(-6)(x-5)
\end{align}
$$

A parabola $(y-k)^2 = 4c(x-h)$ has the focus at a point $(h+c,k)$.
Therefore $(y-3)^2 = 4(-6)(x-5)$ has the focus at the point $(-1, 3)$.

The distance between the point $(-1, 3)$ and the origin $(0,0)$ is :

$$
\begin{align}
\sqrt{ (-1-0)^2 + (3-0)^2 } &= \sqrt{ (-1)^2 + 3^2 } \\
&= \sqrt{ 1+9 } \\
&= \sqrt{ 10 }
\end{align}
$$

So the square of that is $10$.
