$$
\begin{align}
\lim_{ n \to \infty }{\left( \frac{3n+3}{n+2} - \frac{2n+2}{2n+4} \right)^2} 
&= \left( \lim_{ n \to \infty }{ \frac{3n+3}{n+2} - \frac{2n+2}{2n+4} }  \right)^2 \\
&= \left( \lim_{ n \to \infty }{ \frac{n}{n}\frac{3+\frac{3}{n}}{1+\frac{2}{n}} - \frac{n}{n}\frac{2+\frac{2}{n}}{2+\frac{4}{n}} }  \right)^2 \\
&= \left( \lim_{ n \to \infty }{ \frac{3+\frac{3}{n}}{1+\frac{2}{n}} - \frac{2+\frac{2}{n}}{2+\frac{4}{n}} }  \right)^2 \\
&= \left(  \frac{3}{1} - \frac{2}{2}   \right)^2 \\
&= (3-1)^2 \\
&= 2^2 \\
&= 4
\end{align}
$$
