Define $m$ as the following :

$$
\begin{align}
m &= \sqrt{ x+5 }
\end{align}
$$
$$
\begin{align}
5^m &= 25^{m^2} \\
5^m &= (5^{2})^{m^2} \\
5^m &= 5^{2m^2} \\
m &= 2m^2 \\
0 &= 2m^2 - m \\
2m^2 - m &= 0 \\
m(2m-1) &= 0
\end{align}
$$

Therefore $m = 0$ or $2m - 1 = 0$ which means :

$$
\begin{align}
\sqrt{ x+5 } &= 0 \\
x + 5 &= 0 \\
x &= -5
\end{align}
$$

or :

$$
\begin{align}
2m - 1 &= 0 \\
2m &= 1 \\
m &= \frac{1}{2} \\
\sqrt{ x+5 } &= \frac{1}{2} \\
x + 5 &= \frac{1}{4} \\
x &= \frac{1}{4} - 5 \\
x &= \frac{1}{4} - \frac{20}{4} \\
x &= -\frac{19}{4} \\
x &= -4.75
\end{align}
$$
