It is confusing where $(25^0)^3$ actually is. To make it easier for us to solve, We will try put it this way :
$$
\begin{align}
\sqrt{ \sqrt{  \frac{25^0  +\frac{3}{4}}{\frac{7}{256x}}} } &= \sqrt{ \sqrt{ \frac{4x^2+256}{\sqrt{ \left( \frac{120}{5!} \right)^{256} }} } }
\end{align}
$$

We will start by simplifying the innermost expression of both sides.

$$
\begin{align}
\sqrt{ \sqrt{  \frac{(25^0)^3  +\frac{3}{4}}{\frac{7}{256x}}} } &= \sqrt{ \sqrt{ \frac{4x^2+256}{\sqrt{ \left( \frac{120}{5!} \right)^{256} }} } } \\
\sqrt{ \sqrt{  \frac{1  +\frac{3}{4}}{\frac{7}{256x}}} } &= \sqrt{ \sqrt{ \frac{4x^2+256}{\sqrt{ \left( \frac{120}{120} \right)^{256} }} } } \\
\sqrt{ \sqrt{  \left( 1  +\frac{3}{4} \right) \frac{256x}{7} } } &= \sqrt{ \sqrt{ \frac{4x^2+256}{\sqrt{ \left( 1 \right)^{256} }} } } \\
\sqrt{ \sqrt{  \left( \frac{4}{4}  +\frac{3}{4} \right) \frac{256x}{7} } } &= \sqrt{ \sqrt{ \frac{4x^2+256}{\sqrt{ 1 }} } } \\
\sqrt{ \sqrt{  \left( \frac{7}{4} \right) \frac{256x}{7} } } &= \sqrt{ \sqrt{\frac{4x^2+256}{1}} } \\
\sqrt{ \sqrt{  \frac{256x}{4} } } &= \sqrt{ \sqrt{4x^2+256} } \\
\sqrt{ \sqrt{  64x } } &= \sqrt{ \sqrt{4x^2+256} } \\
64x &= 4x^2 + 256 \\
0 &= 4x^2 - 64x + 256 \\
0 &= x^2 - 16x + 64 \\
0 &= x^2 - 8x - 8x + 64 \\
0 &= x(x-8)-8(x-8) \\
0 &= (x-8)(x-8) \\
x - 8 &= 0 \\
x &= 8
\end{align}
$$
