$$
\begin{align}
\frac{\sqrt{ 9x+27}}{2x+10} + \frac{\sqrt{ 9x+27}}{x+5} &= 1 \\
\frac{\sqrt{ 9x+27}}{2x+10} + \frac{2}{2}\frac{\sqrt{ 9x+27}}{(x+5)} &= 1 \\
\frac{\sqrt{ 9x+27}}{2x+10} + \frac{2\sqrt{ 9x+27}}{2(x+5)} &= 1 \\
\frac{\sqrt{ 9x+27}}{2x+10} + \frac{2\sqrt{ 9x+27}}{2x+10} &= 1 \\
\sqrt{9x+27} + 2\sqrt{9x+27} &= 2x + 10 \\
3\sqrt{ 9x+27} &= 2x + 10 \\ 
3\sqrt{ 9(x+3)} &= 2x + 10 \\
3 \sqrt{ 9 }\sqrt{ x+3 } &= 2x + 10 \\
3 \cdot 3 \sqrt{ x+3 } &= 2x + 10 \\
9\sqrt{ x+3 } &= 2x +10 \\
81(x+3) &= (2x+10)^2 \\
81x + 243 &= 4x^2 +40x + 100 \\
0 &= 4x^2 -41x -143 \\
0 &= 4x^2 + 11x - 52x - 143 \\
0 &= x(4x+11)-13(4x+11) \\
0 &= (4x+11)(x-13) \\
\therefore x &= \frac{-11}{4},13 \\
x &= -2.75, 13
\end{align}
$$
