$$
\begin{align}
|3x+5| + |2x-3| &= 25
\end{align}
$$

Try to draw a number line to help with visualizing. We also need to understand the concept of absolute, which is basically the following :

$$
|m| = 
\begin{cases}
m &\text{ ;  if } m \geq 0 \\
-m &\text{ ; if } m < 0
\end{cases}
$$

Define :

$$
\begin{align}
3x + 5 &= m_{1} \\
2x-3 &= m_{2}
\end{align}
$$

Consider when $m_1 \geq 0$ and $m_2 \geq 0$ or $3x+5 \geq 0$ and $2x-3 \geq 0$. That is when 

$$
x \geq -\frac{5}{3} \text{ and } x \geq \frac{3}{2}
$$

Then we can rewrite $|3x+5| + |2x-3| = 25$ as $|m_1| + |m_2| = 25$. Which in the case of both $m_1$ and $m_2$ being greater than zero implies that $|m_1| + |m_2|= m_{1 } + m_{2}= 25$.

$$
\begin{align}
m_{1} + m_{2} &= 25 \\
(3x + 5) + (2x-3) &= 25 \\
5x + 2 &= 25 \\
5x &= 23 \\
x &= \frac{23}{5}
\end{align}
$$

Another case to be considered is when $x \geq \frac{-5}{3}$ and $x < \frac{3}{2}$ (The reason why is because this implies that $m_1 \geq 0$ but $m_2 < 0$).

Then we can rewrite $|m_1| + |m_2| = 25$ as $m_{1} + (-m_{2}) = 25$.

$$
\begin{align}
m_{1} + (-m_{2}) &= 25 \\
m_{1} - m_{2} &= 25 \\
(3x+5) - (2x -3) &= 25 \\
3x + 5 - 2x + 3 &= 25 \\
x + 8 &= 25 \\
x &= 17
\end{align}
$$

But we are considering when $x \geq \frac{-5}{3}$ and $x < \frac{3}{2}$ that implies $x \neq 17$.

And the last case to be considered is when both $m_1$ and $m_2$ are less than zero, which mean $x < \frac{-5}{3}$ and $x < \frac{3}{2}$.

Consider the following as both $m_1$ and $m_2$ are less than zero :

$$
\begin{align} 
|m_{1}| + |m_{2}| &= -m_{1} + (-m_{2})  \\

-m_{1} + (-m_{2}) &= 25 \\
-m_{1} - m_{2} &= 25 \\
-(3x + 5) - (2x -3) &= 25 \\
-3x - 5 - 2x + 3 &= 25 \\
-5x - 2 &= 25 \\
-5x &= 27 \\
x &= \frac{-27}{5}
\end{align}
$$

Therefore $x = \frac{-27}{5}, \frac{23}{5}$.

Therefore $x_{max} + x_{min} = \frac{-27}{5} + \frac{23}{5} = -\frac{4}{5}$
