$$
\begin{align}
\frac{2\log_{3}x - 4}{\log_{3}{\frac{x}{9}}} &= \log_{3}{x^7} - \left( \frac{1}{\log_{x}3} \right)^2 - 8 \\
\end{align}
$$

Define :

$$
m = \log_{3}x
$$

Therefore :

$$
\begin{align}
\frac{2\log_{3}x - 4}{\log_{3}{\frac{x}{9}}} &= \log_{3}{x^7} - \left( \frac{1}{\log_{x}3} \right)^2 - 8 \\
 \frac{2\log_{3}x - 4}{\log_{3}{x} + \log_{3}{\frac{1}{9}}} &= 7\log_{3}{x} - \left( \log_{3}x \right)^2 - 8 \\
 \frac{2\log_{3}x - 4}{\log_{3}{x} + \log_{3}{3^{-2}}} &= 7\log_{3}{x} - \left( \log_{3}x \right)^2 - 8 \\
 \frac{2\log_{3}x - 4}{\log_{3}{x} + (-2\log_{3}{3})} &= 7\log_{3}{x} - \left( \log_{3}x \right)^2 - 8 \\
 \frac{2\log_{3}x - 4}{\log_{3}{x} -2\log_{3}{3}} &= 7\log_{3}{x} - \left( \log_{3}x \right)^2 - 8 \\
 \frac{2m - 4}{m -2} &= 7m - m^2 - 8 \\
 \frac{2(m - 2)}{m -2} &= 7m - m^2 - 8 \\
2 &= - m^2 + 7m - 8 \\
0 &= - m^2 + 7m - 10 \\
m^2 - 7m + 10 &= 0 \\
m^2 - 2m - 5m  + 10 &= 0 \\
m(m-2) - 5(m-2) &= 0 \\
(m-2)(m-5) &= 0 \\
m &= 2, 5
\end{align}
$$

Therefore :

$$
\begin{align}
\log_{3}x &= 2, 5 \\
3^{\log_{3}x} &= 3^2, 3^5 \\
x &= 9, 243
\end{align}
$$

Therefore $x_{min} = 9$.
