$$
\begin{align}
2A - B &= \begin{bmatrix}
-5 &3 \\
4 &7
\end{bmatrix} \\
A - 2B &= \begin{bmatrix}
-5 &4 \\
3 &2
\end{bmatrix}
\end{align}
$$

$$
\begin{align}
\therefore 2A - 4B &= \begin{bmatrix}
-10 &8 \\
6 &4
\end{bmatrix} \\
(2A-B) -(2A-4B) &= \begin{bmatrix}
-5 &3 \\
4 &7
\end{bmatrix} - \begin{bmatrix}
-10 &8 \\
6 &4 
\end{bmatrix} \\
3B &= \begin{bmatrix}
5 &-5 \\
-2 &3
\end{bmatrix} \\
 \\
B &= \begin{bmatrix}
\frac{5}{3} &-\frac{5}{3} \\
-\frac{2}{3} &1
\end{bmatrix} \\
\therefore 2A - B &= \begin{bmatrix}
-5 &3 \\
4 &7
\end{bmatrix} \\
 2A &= \begin{bmatrix}
-5 &3 \\
4 &7
\end{bmatrix} + B \\
2A &= \begin{bmatrix}
-5 &3 \\
4 &7
\end{bmatrix} + \begin{bmatrix}
\frac{5}{3} &-\frac{5}{3} \\
-\frac{2}{3} &1
\end{bmatrix} \\
2A &= \begin{bmatrix}
-\frac{15}{3} &\frac{9}{3} \\
\frac{12}{3} &\frac{21}{3}
\end{bmatrix} + \begin{bmatrix}
\frac{5}{3} &-\frac{5}{3} \\
-\frac{2}{3} & \frac{3}{3}
\end{bmatrix} \\
2A &= \begin{bmatrix}
-\frac{10}{3} &\frac{4}{3} \\
\frac{10}{3} & \frac{24}{3}
\end{bmatrix} \\
A &= \frac{1}{2}\begin{bmatrix}
-\frac{10}{3} &\frac{4}{3} \\
\frac{10}{3} & \frac{24}{3}
\end{bmatrix} \\
A &= \begin{bmatrix}
-\frac{10}{6} &\frac{4}{6} \\
\frac{10}{6} & \frac{24}{6}
\end{bmatrix}
\end{align}
$$


$$
\begin{align}
\det(AB^{-1}) &= \det A \cdot \frac{1}{\det B} \\
&= \frac{\det A }{\det B} \\
&= \frac{\frac{-10}{6} \cdot \frac{24}{6} - \frac{4}{6} \cdot \frac{10}{6}}{\frac{5}{3} - \left( -\frac{5}{3} \right)\left( -\frac{2}{3} \right)} \\
&= \frac{-\frac{240}{36} - \frac{40}{36}}{\frac{5}{3} - \frac{10}{9}} \\
&= \frac{-\frac{280}{36}}{\frac{15}{9}-\frac{10}{9}} \\
&=\frac{-\frac{280}{36}}{\frac{5}{9}} \\
&= -\frac{280}{36} \cdot \frac{{9}}{5} \\
&= -\frac{280}{4} \cdot \frac{1}{5} \\
&= -70 \cdot \frac{1}{5} \\
&= -14
\end{align}
$$
