$$
\begin{align}
a_{2} &= \frac{4}{25} \\
a_{4} &= \frac{16}{625} \\
a_{4} &= a_{2}r^2 \\
\frac{16}{625} &= \frac{4}{25}r^2 \\
\frac{25}{4} \cdot \frac{16}{625} &= r^2 \\
\frac{4}{25} &= r^2 \\
\because r &> 0 \\
\therefore r &= \frac{2}{5} \\
\end{align}
$$


$$
\begin{align}
a_{1} &= \frac{a_{2}}{r} \\
&= \frac{\frac{4}{25}}{\frac{2}{5}} \\
&= \frac{4}{25} \cdot \frac{5}{2} \\
&= \frac{2}{5}
\end{align}
$$


$$
\sum_{i=1}^{\infty}a_{i} = \frac{a_{1}}{1-r}
$$


$$
\begin{align}
\sum_{n=1}^{\infty}a_{n} &= \frac{a_{1}}{1-r} \\
&= \frac{\frac{2}{5}}{1-\frac{2}{5}} \\
&= \frac{\frac{2}{5}}{\frac{5}{5}-\frac{2}{5}} \\
&= \frac{\frac{2}{5} }{\frac{3}{5}} \\
&= \frac{2}{3}
\end{align}
$$
